[llir-semantics] LD and ARG instruction semantics

test/ptr_arith.c
@@ -1,0 +1,8 @@
+
+
+
+void sink_int32(int x);
+
+void arg_to_int64(int *p) {
+  sink_int32((int)p);
+}
