Typing.v
@@ -8,45 +8,10 @@ Require Import Coq.ZArith.ZArith.
 Require Import LLIR.LLIR.
 Require Import LLIR.Maps.
 Require Import LLIR.Values.
+Require Export LLIR.Type.
 
 
 Definition type_env := PTrie.t ty.
-
-Definition ptr_ty := TInt I64.
-Definition syscall_ty := TInt I64.
-
-(* Returns the register defined by an instruction and its type. *)
-Definition get_inst_ty_def (i: inst): option (ty * reg) :=
-  match i with
-  | LLSyscall dst _ _ _ => Some (syscall_ty, dst)
-  | LLCall dst _ _ _ => dst
-  | LLTCall _ _ => None
-  | LLInvoke dst _ _ _ _ => dst
-  | LLTInvoke _ _ _ => None
-
-  | LLArg dst _ _ => Some dst
-  | LLInt8 dst _ _ => Some (TInt I8, dst)
-  | LLInt16 dst _ _ => Some (TInt I16, dst)
-  | LLInt32 dst _ _ => Some (TInt I32, dst)
-  | LLInt64 dst _ _ => Some (TInt I64, dst)
-  | LLMov dst _ _ => Some dst
-
-  | LLFrame dst _ _ _ => Some (ptr_ty, dst)
-  | LLGlobal dst _ _ _ _ => Some (ptr_ty, dst)
-  | LLFunc dst _ _ => Some (ptr_ty, dst)
-
-  | LLLd dst _ _ => Some dst
-  | LLUndef dst _ => Some dst
-  | LLUnop dst _ _ _ => Some dst
-  | LLBinop dst _ _ _ _ => Some dst
-  | LLSelect dst _ _ _ _ => Some dst
-
-  | LLSt _ _ _ => None
-  | LLRet _ => None
-  | LLJcc _ _ _ => None
-  | LLJmp _ => None
-  | LLTrap => None
-  end.
 
 (* Type environment from instructions. *)
 Definition ty_env_inst (insts: inst_map): type_env :=
@@ -79,153 +44,156 @@ Definition well_typed_reg (env: type_env) (r: reg) (t: ty) :=
   env ! r = Some t.
 
 (* Typing rules for binary instructions. *)
-Inductive well_typed_binop: binop -> ty -> ty -> ty -> Prop :=
+Inductive WellTypedBinop: binop -> ty -> ty -> ty -> Prop :=
   | type_cmp:
     forall (t: ty) (dt: ty),
-      well_typed_binop LLCmp t t dt
+      WellTypedBinop LLCmp t t dt
   | type_add:
     forall (t: ty),
-      well_typed_binop LLAdd t t t
+      WellTypedBinop LLAdd t t t
   | type_sll:
     forall (tl: ty_int) (tr: ty_int),
-      well_typed_binop LLSll (TInt tl) (TInt tr) (TInt tl)
+      WellTypedBinop LLSll (TInt tl) (TInt tr) (TInt tl)
   .
 
 (* Typing rules for unary instructions. *)
-Inductive well_typed_unop: unop -> ty -> ty -> Prop :=
-  | type_sext_i32_i64: well_typed_unop LLSext (TInt I32) (TInt I64)
+Inductive WellTypedUnop: unop -> ty -> ty -> Prop :=
+  | type_sext_i32_i64: WellTypedUnop LLSext (TInt I32) (TInt I64)
   .
 
 (* Typing rules for instructions. *)
-Inductive well_typed_inst: type_env -> inst -> Prop :=
+Inductive WellTypedInst: type_env -> inst -> Prop :=
   | type_jmp:
     forall (env: type_env) (target: node),
-      well_typed_inst env (LLJmp target)
+      WellTypedInst env (LLJmp target)
   | type_jcc:
     forall (env: type_env) (cond: reg) (bt: node) (bf: node) (i: ty_int)
       (COND_TY: well_typed_reg env cond (TInt i)),
-      well_typed_inst env (LLJcc cond bt bf)
+      WellTypedInst env (LLJcc cond bt bf)
   | type_ret:
     forall (env: type_env) (ret: reg) (t: ty)
       (RET_TY: well_typed_reg env ret t),
-      well_typed_inst env (LLRet (Some ret))
+      WellTypedInst env (LLRet (Some ret))
   | type_ret_void:
     forall (env: type_env),
-      well_typed_inst env (LLRet None)
+      WellTypedInst env (LLRet None)
   | type_st:
     forall (env: type_env) (next: node) (addr: reg) (val: reg) (t: ty)
       (ADDR_TY: well_typed_reg env addr ptr_ty)
       (VAL_TY: well_typed_reg env val t),
-      well_typed_inst env (LLSt next addr val)
+      WellTypedInst env (LLSt next addr val)
   | type_undef:
     forall (env: type_env) (next: node) (dst: reg) (t: ty)
       (DST_TY: well_typed_reg env dst t),
-      well_typed_inst env (LLUndef (t, dst) next)
+      WellTypedInst env (LLUndef (t, dst) next)
   | type_ld:
     forall (env: type_env) (next: node) (dst: reg) (t: ty) (addr: reg)
       (ADDR_TY: well_typed_reg env addr ptr_ty)
       (DST_TY: well_typed_reg env dst t),
-      well_typed_inst env (LLLd (t, dst) next addr)
+      WellTypedInst env (LLLd (t, dst) next addr)
   | type_frame:
     forall (env: type_env) (dst:reg) (next: node)
       (object: positive) (offset: nat)
       (DST_TY: well_typed_reg env dst ptr_ty),
-      well_typed_inst env (LLFrame dst next object offset)
+      WellTypedInst env (LLFrame dst next object offset)
   | type_global:
     forall (env: type_env) (dst: reg) (next: node)
       (segment: positive) (object: positive) (offset: nat)
       (DST_TY: well_typed_reg env dst ptr_ty),
-      well_typed_inst env (LLGlobal dst next segment object offset)
-  | type_int8:
-    forall (env: type_env) (dst: reg) (next: node) (val: INT.I8.t)
-      (DST_TY: well_typed_reg env dst (TInt I8)),
-      well_typed_inst env (LLInt8 dst next val)
-  | type_int16:
-    forall (env: type_env) (dst: reg) (next: node) (val: INT.I16.t)
-      (DST_TY: well_typed_reg env dst (TInt I16)),
-      well_typed_inst env (LLInt16 dst next val)
-  | type_int32:
-    forall (env: type_env) (dst: reg) (next: node) (val: INT.I32.t)
-      (DST_TY: well_typed_reg env dst (TInt I32)),
-      well_typed_inst env (LLInt32 dst next val)
-  | type_int64:
-    forall (env: type_env) (dst: reg) (next: node) (val: INT.I64.t)
-      (DST_TY: well_typed_reg env dst (TInt I64)),
-      well_typed_inst env (LLInt64 dst next val)
+      WellTypedInst env (LLGlobal dst next segment object offset)
+  | type_int:
+    forall (env: type_env) (dst: reg) (next: node) (val: INT.t) (t: ty)
+      (INT_TY: TypeOfInt val t)
+      (DST_TY: well_typed_reg env dst t),
+      WellTypedInst env (LLInt dst next val)
   | type_arg:
     forall (env: type_env) (t: ty) (dst: reg) (next: node) (idx: nat)
       (DST_TY: well_typed_reg env dst t),
-      well_typed_inst env (LLArg (t, dst) next idx)
+      WellTypedInst env (LLArg (t, dst) next idx)
   | type_binop:
     forall (env: type_env) (op: binop) (next: node)
       (l: reg) (tl: ty) (r: reg) (tr: ty) (dst: reg) (t: ty)
       (LHS_TY: well_typed_reg env l tl)
       (RHS_TY: well_typed_reg env r tr)
       (DST_TY: well_typed_reg env dst t)
-      (OP: well_typed_binop op tl tr t),
-      well_typed_inst env (LLBinop (t, dst) next op l r)
+      (OP: WellTypedBinop op tl tr t),
+      WellTypedInst env (LLBinop (t, dst) next op l r)
   | type_unop:
     forall (env: type_env) (op: unop) (next: node)
       (arg: reg) (argt: ty) (dst: reg) (t: ty)
       (ARG_TY: well_typed_reg env arg argt)
       (DST_TY: well_typed_reg env dst t)
-      (OP: well_typed_unop op argt t),
-      well_typed_inst env (LLUnop (t, dst) next op arg)
+      (OP: WellTypedUnop op argt t),
+      WellTypedInst env (LLUnop (t, dst) next op arg)
   | type_invoke_void:
     forall (env: type_env) (next: node)
       (dst: reg) (t: ty)
       (callee: reg) (args: list reg) (exn: node)
       (CALLEE_TY: well_typed_reg env callee ptr_ty),
-      well_typed_inst env (LLInvoke (Some (t, dst)) next callee args exn)
+      WellTypedInst env (LLInvoke (Some (t, dst)) next callee args exn)
   | type_call_void:
     forall (env: type_env) (next: node)
       (callee: reg) (args: list reg)
       (CALLEE_TY: well_typed_reg env callee ptr_ty),
-      well_typed_inst env (LLCall None next callee args)
+      WellTypedInst env (LLCall None next callee args)
   | type_call:
     forall (env: type_env) (next: node)
       (callee: reg) (args: list reg) (dst: reg) (t: ty)
       (CALLEE_TY: well_typed_reg env callee ptr_ty)
       (DST_TY: well_typed_reg env dst t),
-      well_typed_inst env (LLCall (Some (t, dst)) next callee args)
+      WellTypedInst env (LLCall (Some (t, dst)) next callee args)
   | type_tcall:
     forall (env: type_env)
       (callee: reg) (args: list reg)
       (CALLEE_TY: well_typed_reg env callee ptr_ty),
-      well_typed_inst env (LLTCall callee args)
+      WellTypedInst env (LLTCall callee args)
   | type_syscall:
     forall (env: type_env) (next: node)
       (sno: reg) (args: list reg) (tsno: ty_int) (dst: reg) (t: ty)
       (SNO_TY: well_typed_reg env sno (TInt tsno))
       (DST_TY: well_typed_reg env dst t),
-      well_typed_inst env (LLSyscall dst next sno args)
+      WellTypedInst env (LLSyscall dst next sno args)
   | type_trap:
     forall (env: type_env),
-      well_typed_inst env LLTrap
+      WellTypedInst env LLTrap
   .
 
-Definition well_typed_insts (env: type_env) (insts: inst_map) :=
-  forall (n: node) (i: inst),
-    Some i = insts ! n -> well_typed_inst env i.
+Inductive WellTypedInsts: type_env -> inst_map -> Prop :=
+  | well_typed_insts:
+    forall
+      (env: type_env) (insts: inst_map)
+      (INSTS: forall (n: node) (i: inst), Some i = insts ! n -> WellTypedInst env i),
+        WellTypedInsts env insts.
 
-Inductive well_typed_phi: type_env -> phi -> Prop :=
-  | typed_phi:
+Inductive WellTypedPhi: type_env -> phi -> Prop :=
+  | well_typed_phi:
     forall (env: type_env) (dst: reg) (t: ty) (ins: list (node * reg))
       (INS: forall (n: node) (r: reg), In (n, r) ins -> well_typed_reg env r t),
-      well_typed_phi env (LLPhi (t, dst) ins)
+      WellTypedPhi env (LLPhi (t, dst) ins)
   .
 
-Definition well_typed_phis (env: type_env) (phis: phi_map) :=
-  forall (n: node) (block: list phi) (p: phi),
-    Some block = phis ! n ->
-    In p block ->
-    well_typed_phi env p.
+Inductive WellTypedPhis: type_env -> phi_map -> Prop :=
+  | well_typed_phis:
+    forall
+      (env: type_env) (phis: phi_map)
+      (PHIS:
+        forall (n: node) (block: list phi) (p: phi),
+          Some block = phis ! n ->
+          In p block ->
+          WellTypedPhi env p),
+    WellTypedPhis env phis.
 
-Definition well_typed_func (f: func) :=
-  well_typed_insts (ty_env f) f.(fn_insts)
-  /\
-  well_typed_phis (ty_env f) f.(fn_phis).
+Inductive WellTypedFunc: func -> Prop :=
+  | well_typed_func:
+    forall (f: func)
+      (INSTS: WellTypedInsts (ty_env f) f.(fn_insts))
+      (PHIS: WellTypedPhis (ty_env f) f.(fn_phis)),
+      WellTypedFunc f
+  .
 
-Definition well_typed_prog (p: prog) :=
-  forall (n: name) (f: func),
-    Some f = p ! n -> well_typed_func f.
+Inductive WellTypedProg: prog -> Prop :=
+  | well_typed_prog:
+    forall (p: prog)
+      (FUNCS: forall (n: name) (f: func), Some f = p ! n -> WellTypedFunc f),
+      WellTypedProg p
+  .
