Type.v
@@ -1,0 +1,84 @@
+(* This file is part of the LLIR Semantics project. *)
+(* Licensing information is available in the LICENSE file. *)
+(* (C) 2020 Nandor Licker. All rights reserved. *)
+
+Require Import LLIR.Values.
+
+Inductive ty_int: Type :=
+  | I8
+  | I16
+  | I32
+  | I64
+  | I128
+  .
+
+Inductive ty_float: Type :=
+  | F32
+  | F64
+  | F80
+  .
+
+Inductive ty : Type :=
+  | TInt (i: ty_int)
+  | TFloat (f: ty_float)
+  .
+
+Definition ptr_ty := TInt I64.
+Definition syscall_ty := TInt I64.
+
+Lemma type_dec:
+  forall (t0: ty) (t1: ty),
+    {t0 = t1} + {t0 <> t1}.
+Proof.
+  intros t0 t1.
+  destruct t0; destruct t1; 
+  try destruct i; try destruct i0;
+  try destruct f; try destruct f0;
+  match goal with
+  | [ |- context [ ?a = ?b ] ] => left; reflexivity
+  | [ |- _ ] => right; intros contra; inversion contra
+  end.
+Qed.
+
+(* Returns the type of an integer constant. *)
+Definition type_of_int (v: INT.t): ty :=
+  match v with
+  | INT.Int8 _ => TInt I8
+  | INT.Int16 _ => TInt I16
+  | INT.Int32 _ => TInt I32
+  | INT.Int64 _ => TInt I64
+  end.
+
+(* Type of integers *)
+Inductive TypeOfInt : INT.t -> ty -> Prop :=
+  | ty_of_i8: forall (v: INT.I8.t), TypeOfInt (INT.Int8 v) (TInt I8)
+  | ty_of_i16: forall (v: INT.I16.t), TypeOfInt (INT.Int16 v) (TInt I16)
+  | ty_of_i32: forall (v: INT.I32.t), TypeOfInt (INT.Int32 v) (TInt I32)
+  | ty_of_i64: forall (v: INT.I64.t), TypeOfInt (INT.Int64 v) (TInt I64)
+  .
+
+(* Decidability of TypeOfInt *)
+Lemma TypeOfInt_dec:
+  forall (v: INT.t) (t: ty),
+    {TypeOfInt v t} + {~TypeOfInt v t}.
+Proof.
+  intros v t.
+  destruct v; destruct t;
+    try match goal with
+    | [ |- context [ TFloat _ ]] => right; intros contra; inversion contra
+    end;
+    destruct i;
+    try (left; constructor);
+    right; intros contra;
+    inversion contra.
+Qed.
+
+(* Predicate-Definition Equivalence *)
+Lemma TypeOfInt_type_of_int:
+  forall (v: INT.t) (t: ty),
+    TypeOfInt v t <-> type_of_int v = t.
+Proof.
+  intros v t; split; intros H.
+  - inversion H; constructor.
+  - destruct v; simpl in H; subst; constructor.
+Qed.
